Demo.v
@@ -22,7 +22,7 @@ Definition z := "z".
 Definition negb_app_true :=
     [|
      (\x : Bool =>
-           case x : Bool return Bool of
+           case x : (Bool,[]) return Bool of
            | True -> False
            | False -> True) True
      |].
@@ -49,7 +49,7 @@ Make Definition coq_negb_app_true :=
 Print coq_negb_app_true.
 
 Definition my_negb_syn :=
-  [| \x : Bool => case x : Bool return Bool of
+  [| \x : Bool => case x : (Bool,[]) return Bool of
                    | True -> False
                    | False -> True  |].
 
@@ -70,7 +70,7 @@ Definition is_zero_syn :=
   [|
 
       \x : Nat =>
-           case x : Nat return Bool of
+           case x : (Nat,[]) return Bool of
            | Z -> True
            | Suc y -> False
 
@@ -83,7 +83,7 @@ Definition pred_syn :=
   [|
 
       \x : Nat =>
-           case x : Nat return Nat of
+           case x : (Nat,[]) return Nat of
            | Z -> x
            | Suc y -> y
 
@@ -115,7 +115,7 @@ Compute (expr_eval_n Σ' 5 [] prog3).
 Definition factorial_syn :=
   [|
    fix "factorial" (x : Nat) : Nat :=
-       case x : Nat return Nat of
+       case x : (Nat,[]) return Nat of
        | Z -> 1
        | Suc y -> x * ("factorial" y)
   |].
@@ -126,7 +126,7 @@ Make Definition factorial :=
 Definition plus_syn : expr :=
   [| fix "plus" (x : Nat) : Nat -> Nat :=
        \y : Nat =>
-           case x : Nat return Nat of
+           case x : (Nat,[]) return Nat of
            | Z -> y
            | Suc z -> Suc ("plus" z y) |].
 
@@ -157,12 +157,12 @@ Parameter bbb: bool.
 Quote Definition two_arg_fun_app_syn' := ((fun (x : nat) (_ : bool) => x) 1 bbb).
 
 Example one_plus_one_two : expr_eval_n Σ 10 [] one_plus_one = Ok two.
-Proof. reflexivity. Qed.
+Proof.  reflexivity. Qed.
 
 Definition plus_syn' :=
   [| \x : Nat =>
           (fix "plus" (y : Nat) : Nat :=
-           case y : Nat return Nat of
+           case y : (Nat,[]) return Nat of
            | Z -> x
            | Suc z -> Suc ("plus" z))
   |].
@@ -197,7 +197,7 @@ Qed.
 
 Definition id_rec :=
   [| (fix "plus" (y : Nat) : Nat :=
-           case y : Nat return Nat of
+           case y : (Nat,[]) return Nat of
            | Z -> 0
            | Suc z -> Suc ("plus" z))
    |].
